more Zip loop

Given_Clause_Loops/Prover_Lazy_List_Queue.thy
@@ -15,7 +15,7 @@ begin
 
 subsection \<open>Locales\<close>
 
-locale prover_lqueue =
+locale prover_lazy_list_queue =
   fixes
     empty :: 'q and
     add_llist :: "'e llist \<Rightarrow> 'q \<Rightarrow> 'q" and
@@ -26,6 +26,7 @@ locale prover_lqueue =
     llists_empty[simp]: "llists empty = {#}" and
     llists_not_empty: "Q \<noteq> empty \<Longrightarrow> llists Q \<noteq> {#}" and
     llists_add[simp]: "llists (add_llist es Q) = llists Q + {#es#}" and
+    llist_remove[simp]: "llists (remove_llist es Q) = llists Q - {#es#}" and
     llists_pick_elem: "(\<exists>es. es \<noteq> LNil \<and> es \<in># llists Q) \<Longrightarrow>
       \<exists>e es. LCons e es \<in># llists Q \<and> fst (pick_elem Q) = e
         \<and> llists (snd (pick_elem Q)) = llists Q - {#LCons e es#} + {#es#}"
@@ -50,7 +51,8 @@ inductive pick_lqueue_step :: "'q \<Rightarrow> 'q \<Rightarrow> bool" where
 
 end
 
-locale fair_prover_lqueue = prover_lqueue empty add_llist remove_llist pick_elem llists
+locale fair_prover_lazy_list_queue =
+  prover_lazy_list_queue empty add_llist remove_llist pick_elem llists
   for
     empty :: 'q and
     add_llist :: "'e llist \<Rightarrow> 'q \<Rightarrow> 'q" and
@@ -61,6 +63,30 @@ locale fair_prover_lqueue = prover_lqueue empty add_llist remove_llist pick_elem
     enat i < llength Qs \<Longrightarrow> LCons e es \<in># llists (lnth Qs i) \<Longrightarrow>
     \<exists>j \<ge> i. enat (Suc j) < llength Qs \<and> pick_lqueue_step_aux (lnth Qs j) e es (lnth Qs (Suc j))"
 begin
+end
+
+
+subsection \<open>Instantiation with FIFO Queue\<close>
+
+text \<open>As a proof of concept, we show that a FIFO queue can serve as a fair
+prover lazy list queue.\<close>
+
+locale fifo_prover_lazy_list_queue
+begin
+
+fun pick_elem :: "'e llist list \<Rightarrow> 'e \<times> 'e llist list" where
+  "pick_elem [] = undefined"
+| "pick_elem (LNil # ess) = pick_elem ess"
+| "pick_elem (LCons e es # ess) = (e, es # ess)"
+
+sublocale prover_lazy_list_queue "[]" "\<lambda>es ess. ess @ [es]" remove1 pick_elem mset
+proof
+  show "\<And>Q. \<exists>es. es \<noteq> LNil \<and> es \<in># mset Q \<Longrightarrow>
+    \<exists>e es. LCons e es \<in># mset Q \<and> fst (pick_elem Q) = e
+      \<and> mset (snd (pick_elem Q)) = mset Q - {#LCons e es#} + {#es#}"
+    sorry
+qed simp+
+
 end
 
 end
